inputs

Spacetalk/SimpleArith.lean
@@ -3,16 +3,14 @@ import Mathlib.Data.Stream.Defs
 import Spacetalk.Vector
 
 inductive Exp : Nat → Type
-  | val : Nat → Exp 0
-  | var : Exp 1
-  | plus : Exp inp1 → Exp inp2 → Exp (inp1 + inp2)
+  | val : Nat → Exp n
+  | var : Fin n → Exp n
+  | plus : Exp n → Exp n → Exp n
 
-def Exp.eval : Exp inp → Vector Nat inp → Nat
-| (.val v), _ => v
-| .var, inp => inp[0]
-| (.plus e1 e2), inp =>
-  let (inp1, inp2) := inp.split
-  (e1.eval inp1) + (e2.eval inp2)
+def Exp.eval : Exp n → Vector Nat n → Nat
+| val v, _ => v
+| var idx, inp => inp[idx]
+| plus e1 e2, inp => (e1.eval inp) + (e2.eval inp)
 
 def Vector.packStreams (ss : Vector (Stream' α) len) : Stream' (Vector α len) :=
   λ n => ss.map (·.get n)
@@ -23,90 +21,95 @@ def Exp.denote (e : Exp inp) (inpVals : Vector (Stream' Nat) inp) : Stream' Nat 
 -- single output only
 inductive Node (α : Type) : Nat → Type
   | id : Node α 1
-  | val : Nat → Node α 0
+  | const : Nat → Node α 0
   | plus : Node α 2
 
 inductive Graph (α : Type) : Nat → Type
-  | nodeClosed : Node α inp → Vector α inp → Graph α 0
+  | var : α → (α → Graph α n) → Graph α n
+  | node : Node α inp → Vector α inp → Graph α 0
   | μClosed : Node α inp → Vector α inp → (α → Graph α n) → Graph α n
-  | μOpen : Node α inp → (α → Graph α n) → Graph α (inp + n)
+  | μOpenLeft : Node α inp → (α → Graph α n) → Graph α (inp + n)
+  | μOpenRight : Node α inp → (α → Graph α n) → Graph α (n + inp)
 
 def Node.denote : Node α inp → (Vector (Stream' Nat) inp → Stream' Nat)
-| .id => λ v => v[0]
-| .val v => λ _ => .const v
-| .plus => λ inp => Stream'.zip HAdd.hAdd inp[0] inp[1]
+| id => λ v => v[0]
+| const v => λ _ => .const v
+| plus => λ inp => Stream'.zip HAdd.hAdd inp[0] inp[1]
 
 def Graph.denote : Graph (Stream' Nat) nInp → (Vector (Stream' Nat) nInp) → Stream' Nat
-| (.nodeClosed n inp), _ => n.denote inp
-| (.μClosed n μInp f), fInp => (f (n.denote μInp)).denote fInp
-| (.μOpen n f), vInp =>
+| var s c, inp => (c s).denote inp
+| node n inp, _ => n.denote inp
+| μClosed n μInp f, fInp => (f (n.denote μInp)).denote fInp
+| μOpenLeft n f, vInp =>
   let (μNodeInp, fInp) := vInp.split
   (f (n.denote μNodeInp)).denote fInp
+| μOpenRight n f, vInp =>
+  let (fInp, μNodeInp) := vInp.split
+  (f (n.denote μNodeInp)).denote fInp
 
-def Exp.compileC (cont : α → Graph α nCont) : Exp nExp → Graph α (nExp + nCont)
-| .val v => (Nat.zero_add nCont).symm ▸ .μClosed (.val v) #v[] cont
-| .var => .μOpen .id cont
-| @Exp.plus inp1 inp2 e1 e2 =>
-  have : inp1 + (inp2 + nCont) = inp1 + inp2 + nCont := by omega
-  this ▸
-    (e1.compileC λ e1Out =>
-     e2.compileC λ e2Out =>
-     .μClosed .plus #v[e1Out, e2Out] cont)
+def addInputs : (n : Nat) → (Vector α n → Graph α 0) → Graph α n
+| 0, c => c #v[]
+| n + 1, c =>
+  .μOpenRight .id λ last =>
+  addInputs n λ front =>
+  c (front.push last)
+
+def Exp.compileC (inputs : Vector α n) (cont : α → Graph α 0) : Exp n → Graph α 0
+| val v => .μClosed (.const v) #v[] cont
+| var idx => .var inputs[idx] cont
+| plus e1 e2 =>
+  e1.compileC inputs λ e1Out =>
+  e2.compileC inputs λ e2Out =>
+  .μClosed .plus #v[e1Out, e2Out] cont
+
+def Exp.compile (e : Exp n) : Graph α n :=
+  addInputs n λ inputs =>
+  e.compileC inputs λ out => .node .id #v[out]
 
 theorem graph_cast_denote {n m : Nat} {h : n = m} {g1 : Graph (Stream' Nat) n} {inp : Vector (Stream' Nat) m}
   : (h ▸ g1).denote inp = g1.denote (h ▸ inp) := by
   subst h
   simp_all only
 
-def Exp.compile (e : Exp n) : Graph α n :=
-  e.compileC λ out => .nodeClosed .id #v[out]
-
-theorem compileC_correct
-  : ∀ e : Exp nExp, ∀ c : Stream' Nat → Graph _ nCont,
-    ∀ vInpExp : Vector (Stream' Nat) nExp, ∀ vInpCont : Vector (Stream' Nat) nCont,
-    (c (e.denote vInpExp)).denote vInpCont = (e.compileC c).denote (vInpExp ++ vInpCont) := by
-  intro e c vInpExp vInpCont
-  induction e generalizing c nCont with
-  | val v =>
-    -- Get rid of all castings first
-    simp only [Exp.compileC, graph_cast_denote]
-    conv =>
-      rhs
-      arg 2
-      simp only [Vector.nil_append, Eq.rec_eq_cast, cast_cast, cast_eq]
-    -- rfl closes the goal now
-    rfl
-  | var =>
+lemma compileC_correct
+  : ∀ e : Exp n, ∀ c : Stream' Nat → Graph _ 0,
+    ∀ inpVec : Vector (Stream' Nat) n,
+    (c (e.denote inpVec)).denote = (e.compileC inpVec c).denote := by
+  intro e c inpVec
+  induction e generalizing c with
+  | val v => rfl
+  | var idx =>
     unfold Exp.denote
-    simp only [Exp.eval, Vector.packStreams, Vector.getElem_map, Exp.compileC, Graph.denote,
-      Node.denote, Vector.append_split_left_eq, Vector.append_split_right_eq]
+    simp only [Exp.eval, Vector.packStreams, Fin.getElem_fin, Vector.getElem_map, Exp.compileC,
+      Graph.denote]
     rfl
   | plus e1 e2 ih1 ih2 =>
-    -- Get rid of all casts
-    simp only [Exp.compileC, graph_cast_denote]
-    obtain ⟨vInp1, vInp2, h_inp⟩ := Vector.add_eq_append vInpExp
-    rw [h_inp]
-    conv =>
-      rhs
-      arg 2
-      simp only [Vector.append_assoc, Eq.rec_eq_cast, cast_cast, cast_eq]
-    -- No more casts!
-    rw [←(ih1 _ vInp1)]
-    rw [←(ih2 _ vInp2)]
-    simp only [Graph.denote, Node.denote, Vector.getElem_mk, List.getElem_toArray,
-      List.getElem_cons_zero, List.getElem_cons_succ]
-    unfold Stream'.zip
-    unfold Exp.denote
-    simp only [Exp.eval, Vector.packStreams, Vector.append_split_map_left_eq,
-      Vector.append_split_map_right_eq]
-    subst h_inp
+    simp only [Exp.compileC]
+    rw [←ih1]
+    rw [←ih2]
     rfl
 
-theorem compile_correct : ∀ e : Exp nExp, e.denote = e.compile.denote := by
+lemma addInputs_eq
+  : ∀ n, ∀ c : Vector (Stream' Nat) n → Graph _ 0, ∀ inpVec : Vector (Stream' Nat) n,
+    (c inpVec).denote #v[] = (addInputs n λ inputs => c inputs).denote inpVec := by
+  intro n
+  induction n with
+  | zero =>
+    intro c inpVec
+    simp only [Vector.size_zero_eq, addInputs]
+  | succ n ih =>
+    intro c inpVec
+    simp [addInputs, Graph.denote, Node.denote]
+    rw [←ih]
+    rw [Vector.split_last_push_eq]
+
+theorem compile_correct : ∀ e : Exp n, e.denote = e.compile.denote := by
   intro e
   funext inp
   simp only [Exp.compile]
-  have := compileC_correct e (λ out => .nodeClosed .id #v[out]) inp #v[]
-  rw [Vector.append_nil] at this
-  rw [←this]
-  rfl
+  have := compileC_correct e (λ out => .node .id #v[out]) inp
+  simp only [Graph.denote] at this
+  have := congr (a₁ := #v[]) this rfl
+  simp only [Node.denote, Vector.getElem_mk, List.getElem_toArray, List.getElem_cons_zero] at this
+  rw [this]
+  rw [←addInputs_eq]
